Ite.v
@@ -21,22 +21,63 @@ Require Import Coq.micromega.Lia.
 Module IteGadget(PF: GaloisField).
   Import PF.
   Include Gadget PF.
-  Import VectorNotations.
+  Import ListNotations.
 
   (** Example 1: Division *)
   Definition ite :=
-    <{ \_: Bool * Field * Field,
-           if fst #0 then fst (snd #0) else snd (snd #0)
+    <{ \_: Bool, \_: Field, \_: Field,
+           if #2 then #1 else #0
      }>. 
 
   Definition ite_check :=
-    <[ { (1i[0]) * (1i[2] + -1i[1]) == (1o[0] + -1i[1]) } ]>.
+    <[ { (1i[0]) * (1i[2] + -1i[1]) == (1o + -1i[1]) } ]>.
 
-   (** Second equivalence proof over r1cs *)
+
+  Ltac typer1 :=
+    match goal with
+    | [|- <{{ _ |- <{ \_ : _, _ }> :: _}}>] => eapply typing_abs; intros; cbn
+    | [|- <{{ _ |- <{ if _ then _ else _ }> :: _ }}>] => eapply typing_if; constructor; cbn
+    | [|- (?x, ?T) = (?x, ?T) \/ _] => left; reflexivity
+    | [|- _ \/ (?x, ?T) = (?x, ?T) ] => right; reflexivity
+    | [|- _ \/ (?x1, ?T1) = (?x2, ?T2) ] => left
+    | [|- (?x1, ?T1) = (?x2, ?T2) \/ _ ] => right
+    | [|- uniq _ ] => repeat constructor; eassumption
+    end.
+
+  (** Second equivalence proof over r1cs *)
   Theorem ite_equiv_r1cs:
     ite <=*=> ite_check.
   Proof.
-    unfold ite_check, r1cs_lambda_equiv, ite.
+    unfold ite_check, ite.
+    apply Step with (t:=<{{ Bool }}>) (t':=<{{Field -> Field -> Field}}>).
+    - constructor.
+    - repeat typer.
+    - constructor.
+    - intros.
+      apply Step with (t:=<{{ Field }}>) (t':=<{{Field -> Field}}>).
+      + constructor.
+      + apply typing_app with (T1:=<{{ Bool }}>).
+        
+        cbn.
+        right.
+        right.
+        left.
+        reflexivity.
+        repeat constructor; eassumption.
+      + constructor.
+        cbn.
+        
+        repeat (constructor; eassumption).
+    - econstructor.
+      intros x H. 
+      econstructor; intros; cbn.      
+      econstructor; intros; cbn.
+      econstructor; intros; cbn.
+      econstructor; intros; cbn.
+      right.
+      right.
+      econstructor. repeat econstructor. eassumption.
+      repeat econstructor; eassumption.
     intros.
     cbn in vars, inps, outs, HcannonIn, HcannonOut.
     unfold correct, correct_lt.
