R1cs.v
@@ -11,25 +11,47 @@ Import Z.
 Require Import Coq.Init.Nat.
 Require Import Coq.Vectors.VectorDef.
 Require Import Coq.Vectors.Fin.
+Require Import Coq.micromega.Lia.
 
 Set Implicit Arguments.
 Set Printing Implicit.
+Set Transparent Obligations.
 
 Module R1CS(PF: GaloisField).
   Import PF.
   Import VectorNotations.
+  Import ListNotations.
+ 
   Definition Vfp := Vector.t Fp.
   
+  Class Computable a := {
+    (** With more inputs/vars *)
+    eval_lt{i v i' v'}(circ: a i v)(inputs: Vfp i')(vars: Vfp v')(out: Fp): i <= i' -> v <= v' -> list Fp;
+    
+    (** With exact inputs/vars *)
+    eval{i v}(circ: a i v)(inputs: Vfp i)(vars: Vfp v)(out: Fp): list Fp :=
+      eval_lt circ inputs vars out (Nat.le_refl i)(Nat.le_refl v);
+    
+    (** Substitute the 0th input with val *)
+    substitute{i v}(circ: a i v)(val: Fp): a (i-1)%nat v;
+
+    (** Does it sum to zero *)
+    correct{i v}(circ: a i v)(inputs: Vfp i)(vars: Vfp v)(out: Fp): Prop :=
+      let values := eval circ inputs vars out in
+      List.Forall (fun v => v = 0:%p) values
+                                       }.
+
+  (** R1CS language definition *)
   Inductive term: nat -> nat -> Set :=
-  | input: forall (n: nat), term (S n) 0
-  | output: term 0 0
-  | var: forall (n: nat), term 0 (S n)
-  | one: term 0 0.
+  | input(m: Fp): forall (n: nat), term (S n) 0
+  | output(m: Fp): term 0 0
+  | var(m: Fp): forall (n: nat), term 0 (S n)
+  | one(m: Fp): term 0 0.
 
   Inductive additions: nat -> nat -> Type :=
-  | ahead: forall i v, Fp * term i v -> additions i v
+  | ahead: forall i v, term i v -> additions i v
   | atail: forall i v i' v',
-      Fp * term i v ->
+      term i v ->
       additions i' v' ->
       additions (max i i') (max v v').
   
@@ -40,34 +62,38 @@ Module R1CS(PF: GaloisField).
       (C: additions i'' v''),
       constraint (max i (max i' i'')) (max v (max v' v'')).
 
-  Inductive r1cs: nat -> nat -> nat -> Type :=
-  | rnil: r1cs 0 0 0
-  | rcons: forall n i v i' v',
+  Inductive r1cs: nat -> nat -> Type :=
+  | rhead: forall i v, constraint i v -> r1cs i v
+  | rtail: forall i v i' v',
       constraint i v ->
-      r1cs n i' v' ->
-      r1cs (S n) (max i i') (max v v').
+      r1cs i' v' ->
+      r1cs (max i i') (max v v').
   
   Arguments additions {i} {v}.
   Arguments ahead {i} {v}.
   Arguments atail {i} {v} {i'} {v'}.
   Arguments constraint {i} {v}.
   Arguments lc {i} {v} {i'} {v'} {i''} {v''}.
-  Arguments rcons {n} {i} {v} {i'} {v'}.
-  Arguments r1cs {n} {i} {v}.
+  Arguments rhead {i} {v}.
+  Arguments rtail {i} {v} {i'} {v'}.
+  Arguments r1cs {i} {v}.
   
   Definition r1cs_singleton{i v}(c: @constraint i v) :=
-    rcons c rnil.
+    rhead c.
 
   (** syntax *)
   Declare Custom Entry r1cs.
-  
-  Notation "<[ x ; .. ; y ]>" :=
-    (rcons x .. (rcons y rnil) ..)
-      (at level 1,
-          x custom r1cs at level 2,
-          y custom r1cs at level 2,
-          left associativity).
 
+  Notation "<[ a ]>" :=
+    (rhead a) (at level 1, a custom r1cs at level 2).
+  
+  Notation "<[ a1 ; .. ; a2 ; a3 ]>" :=
+    (rtail a1 .. (rtail a2 (rhead a3)) ..)
+      (at level 1,
+       a1 custom r1cs at level 2,
+       a2 custom r1cs at level 2,
+       a3 custom r1cs at level 2).
+  
   Notation "'{' a '*' b '==' c '}'" :=
     (lc a b c)
       (in custom r1cs at level 2,
@@ -87,24 +113,24 @@ Module R1CS(PF: GaloisField).
           a3 custom r1cs at level 4).
   
   Notation "z 'i[' n ']'" :=
-    (to_p z, input n%nat)
+    (input (to_p z) n%nat)
       (in custom r1cs at level 4,
           n constr,
           z constr).
   
   Notation "z 'o'" :=
-    (to_p z, output)
+    (output (to_p z))
       (in custom r1cs at level 4,
           z constr).
   
   Notation "z 'v[' n ']'" :=
-    (to_p z, var n%nat)
+    (var (to_p z) n%nat)
       (in custom r1cs at level 4,
           n constr,
           z constr).
 
   Notation "[ z ]" :=
-    (to_p z, one)
+    (one (to_p z))
       (in custom r1cs at level 4,
           z constr at level 0).
 
@@ -113,39 +139,41 @@ Module R1CS(PF: GaloisField).
                 { (3o + 3i[1]) * (3i[0] + 2v[2]) == ([1]) };
               { (3o + 3i[1]) * (3i[0] + 2v[2]) == ([1]) }  ]>.   
 
+
   Fixpoint eval_additions{i v i' v'}
            (adds: @additions i v)
            (inputs: Vfp i')
-           (output: Fp)
-           (vars: Vfp v'): i <= i' -> v <= v' -> Fp.
+           (vars: Vfp v')
+           (output: Fp): i <= i' -> v <= v' -> Fp.
     invert adds; intros.
-    - invert H; invert H3.
+    - invert H.
       + apply le_lt_Sn_m in H0.
-        exact (pkmul H2 (Vector.nth inputs (Fin.of_nat_lt H0))).  (** Fp * Input term *)
-      + exact (pkmul H2 output). (** Fp * Output term *)
+        exact (pkmul m (Vector.nth inputs (Fin.of_nat_lt H0))).  (** Fp * Input term *)
+      + exact (pkmul m output). (** Fp * Output term *)
       + apply le_lt_Sn_m in H1.
-        exact (pkmul H2 (Vector.nth vars (Fin.of_nat_lt H1))).    (** Fp * Var term *)
-      + exact H2. (** Fp * 1 (One) term *)
-    - specialize (eval_additions _ _ _ _ H0 inputs output vars) as Hprev.
+        exact (pkmul m (Vector.nth vars (Fin.of_nat_lt H1))).    (** Fp * Var term *)
+      + exact m. (** Fp * 1 (One) term *)
+    - specialize (eval_additions _ _ _ _ H0 inputs vars output) as Hprev.
       pose proof (Nat.max_lub_r _ _ _ H1).
       pose proof (Nat.max_lub_r _ _ _ H2).
       pose proof (Nat.max_lub_l _ _ _ H1).
       pose proof (Nat.max_lub_l _ _ _ H2).
       clear H1 H2.
-      invert H; invert H2.
+      invert H.
       + apply le_lt_Sn_m in H5.
-        exact (pkplus (Hprev H3 H4) (pkmul H1 (Vector.nth inputs (Fin.of_nat_lt H5)))).
-      + exact (pkplus (Hprev H3 H4) (pkmul H1 output)).
+        exact (pkplus (Hprev H3 H4) (pkmul m (Vector.nth inputs (Fin.of_nat_lt H5)))).
+      + exact (pkplus (Hprev H3 H4) (pkmul m output)).
       + apply le_lt_Sn_m in H6.
-        exact (pkplus (Hprev H3 H4) (pkmul H1 (Vector.nth vars (Fin.of_nat_lt H6)))).
-      + exact (pkplus (Hprev H3 H4) H1).
+        exact (pkplus (Hprev H3 H4) (pkmul m (Vector.nth vars (Fin.of_nat_lt H6)))).
+      + exact (pkplus (Hprev H3 H4) m).
   Defined.
 
+  
   Fixpoint eval_constraint{i v i' v'}
            (ctr: @constraint i v)
            (inputs: Vfp i')
-           (output: Fp)
-           (vars: Vfp v') : i <= i' -> v <= v' -> Fp.
+           (vars: Vfp v')
+           (output: Fp): i <= i' -> v <= v' -> Fp.
     invert ctr.
     intros.
     pose proof (Nat.max_lub_r _ _ _ H).
@@ -157,57 +185,97 @@ Module R1CS(PF: GaloisField).
     pose proof (Nat.max_lub_r _ _ _ H2).
     pose proof (Nat.max_lub_l _ _ _ H2).
     clear H H0 H1 H2.
-    pose proof (eval_additions A inputs output vars H4 H5) as SumA.
-    pose proof (eval_additions B inputs output vars H6 H8) as SumB.
-    pose proof (eval_additions C inputs output vars H3 H7) as SumC.
+    pose proof (eval_additions A inputs vars output H4 H5) as SumA.
+    pose proof (eval_additions B inputs vars output H6 H8) as SumB.
+    pose proof (eval_additions C inputs vars output H3 H7) as SumC.
     exact (pksub (pkmul SumA SumB) SumC). (** A * B - C *)
   Defined.
-
-  Import VectorNotations.
-  Fixpoint eval_fix{n i v i' v'}
-           (r: @r1cs n i v)
+  
+  Fixpoint eval_fix{i v i' v'}
+           (r: @r1cs i v)
            (inputs: Vfp i')
-           (output: Fp)
-           (vars: Vfp v'): i <= i' -> v <= v' -> Vfp n.
+           (vars: Vfp v')
+           (output: Fp) : i <= i' -> v <= v' -> list Fp.
   Proof.
     intros.
     invert r.
-    - exact [].
+    - pose proof (eval_constraint H1 inputs vars output H H0) as Hhead.
+      exact [Hhead]%list.
     - pose proof (Nat.max_lub_r _ _ _ H).
       pose proof (Nat.max_lub_l _ _ _ H).
       pose proof (Nat.max_lub_r _ _ _ H0).
       pose proof (Nat.max_lub_l _ _ _ H0).
-      pose proof (eval_fix _ _ _ _ _ H2 inputs output vars H3 H5) as Hprev.
-      pose proof (eval_constraint H1 inputs output vars H4 H6) as CtrEval.
-      exact (CtrEval :: Hprev). 
+      pose proof (eval_fix _ _ _ _ H2 inputs vars output H3 H5) as Hprev.
+      pose proof (eval_constraint H1 inputs vars output H4 H6) as CtrEval.
+      exact (CtrEval :: Hprev)%list.
   Defined.
 
-  Definition eval{n i v i' v'}
-             (r: @r1cs n i v)(inputs: Vfp i')(output: Fp)(vars: Vfp v')
-             {Hi: i <= i'} {Hv: v <= v'} :=
-    @eval_fix n i v i' v' r inputs output vars Hi Hv.
+  (** Substitute [v / inp[1]], and [inp[n] / inp[S n]] *)
+
+  Definition substitute_inp{i v}(a: @term i v)(n: Fp): @term (i-1) v :=
+    match a in (@term n v) return (@term (n-1) v) with
+    | input m 0 => one (pkmul m n)
+    | input m (S a) => input m a
+    | output m => output m
+    | var m n => var m n
+    | one m => one m
+    end.
+
+  Program Fixpoint substitute_additions{i v}(a: @additions i v)(inp: Fp): @additions (i-1) v :=
+    match a with
+    | ahead h => ahead (substitute_inp h inp)
+    | atail h ts => atail (substitute_inp h inp) (substitute_additions ts inp)
+    end.
+  Next Obligation. apply Nat.sub_max_distr_r. Defined.
+
+  Program Fixpoint substitute_constraint{i v}(ctr: @constraint i v)(v: Fp) :=
+    match ctr in @constraint i v return (@constraint (i-1) v) with
+    | lc a b c =>
+      lc (substitute_additions a v) (substitute_additions b v) (substitute_additions c v)
+    end.
+  Next Obligation. rewrite Nat.sub_max_distr_r; apply Nat.sub_max_distr_r. Defined.
+
+  Program Fixpoint substitute_r1cs{i v}(r: @r1cs i v)(k: Fp): @r1cs (i-1) v :=
+    match r with
+    | rhead c => rhead (substitute_constraint c k)
+    | rtail h ts => rtail (substitute_constraint h k) (substitute_r1cs ts k)
+    end.
+  Next Obligation. apply Nat.sub_max_distr_r. Defined.
+
+  (** Use those as the public interface to r1cs *)
+  Instance Computable_additions: Computable (@additions) :=
+    {
+    eval_lt{i v i' v'}(circ: @additions i v)(inputs: Vfp i')(vars: Vfp v')(out: Fp) :=
+      fun Hi Hv => [ @eval_additions i v i' v' circ inputs vars out Hi Hv]%list;
+
+    substitute := @substitute_additions
+    }.
+
+  Instance Computable_constraint: Computable (@constraint) :=
+    {
+    eval_lt{i v i' v'}(circ: @constraint i v)(inputs: Vfp i')(vars: Vfp v')(out: Fp) :=
+      fun Hi Hv => [ @eval_constraint i v i' v' circ inputs vars out Hi Hv]%list;
+    
+    substitute := @substitute_constraint
+    }.
   
-  Definition correct_lt{n i v i' v'}
-             (r: @r1cs n i v)(inputs: Vfp i')(output: Fp)(vars: Vfp v')
-             {Hi: i <= i'}{Hv: v <= v'}: Prop :=
-    let values := @eval n i v i' v' r inputs output vars Hi Hv in
-    Vector.Forall (fun v => v = 0:%p) values.
-
-  Definition correct{n i v}(r: @r1cs n i v)(inputs: Vfp i)(output: Fp)(vars: Vfp v): Prop :=
-    @correct_lt n i v i v r inputs output vars (Nat.le_refl i)(Nat.le_refl v).
-
-  Import VectorNotations.
-  Unset Printing Implicit.
+  Instance Computable_r1cs: Computable (@r1cs) :=
+    {
+    eval_lt := @eval_fix;
+    
+    substitute := @substitute_r1cs
+    }.
+  
   Lemma example_correct1:
-    correct <[ { (1i[0]) * (1i[1]) == (1o) } ]> [1:%p; 1:%p] (1:%p) [].
+    correct <[ { (1i[0]) * (1i[1]) == (1o) } ]> [1:%p; 1:%p] [] (1:%p).
   Proof.
-    unfold correct, correct_lt.
+    unfold correct.
     cbn.
     constructor.
     destruct FTH.
     inversion F_R.
     - autorewrite with pk using trivial.
     - constructor.
-  Qed.
+  Defined.
 
 End R1CS.
